src/Dafny/examples/fs/dir_fs.dfy
@@ -30,6 +30,7 @@ module DirFs
     // domain is just the inodes that are allocated directories
     ghost var dirents: map<Ino, Dirents>
     const fs: ByteFilesys<()>
+    const rootIno: Ino
 
     const Repr: set<object> := {this} + fs.Repr
 
@@ -44,30 +45,144 @@ module DirFs
       reads Repr
     {
       && alloc_ino_dom(fs.fs.inode_owner(), data)
-      && forall ino:Ino :: ino in dirents <==>
-        (fs.fs.inode_owner()[ino].Some? && fs.inode_types()[ino].DirType?)
+      && (forall ino:Ino :: ino in dirents <==>
+        (fs.fs.inode_owner()[ino].Some? && fs.inode_types()[ino].DirType?))
+    }
+
+    predicate ValidRoot()
+      reads Repr
+      requires fs.Valid()
+    {
+      // the root inode is allocated and is actually a directory
+      && fs.fs.inode_owner()[rootIno].Some?
+      && fs.inode_types()[rootIno].DirType?
     }
 
     predicate ValidDirents()
+      requires fs.Valid()
       reads Repr
     {
-      // relate fs.data() to dirents
-      true
+      forall ino:Ino | ino in dirents ::
+        fs.data()[ino] == dirents[ino].enc()
     }
+
+    predicate {:opaque} ValidFiles()
+      requires fs.Valid()
+      reads Repr
+    {
+      forall ino:Ino | fs.fs.inode_owner()[ino].Some? && fs.inode_types()[ino].FileType? ::
+           ino in data && data[ino] == ByteFile(fs.data()[ino])
+    }
+
+    predicate {:opaque} ValidDirs()
+      requires fs.Valid()
+      reads Repr
+    {
+
+      forall ino:Ino | ino in dirents :: ino in data && data[ino] == DirFile(dirents[ino].dir)
+    }
+
+    predicate ValidData()
+      requires fs.Valid()
+      reads Repr
+    {
+      && ValidFiles()
+      && ValidDirs()
+    }
+
+    predicate ValidUnusedInodes()
+      requires fs.Valid()
+      reads Repr
+    {
+      forall ino:Ino | fs.fs.inode_owner()[ino].None? ::
+        fs.inode_types()[ino].FileType? && fs.data()[ino] == []
+    }
+
 
     predicate Valid()
       reads Repr
     {
       && fs.Valid()
       && ValidDomains()
+      && ValidRoot()
+      && ValidDirents()
+      && ValidData()
+      && ValidUnusedInodes()
     }
 
-    constructor Init(d: Disk)
+    constructor Init(fs: ByteFilesys<()>, rootIno: Ino)
+      requires fs.Valid()
+      requires fs.data() == map ino: Ino {:trigger} :: if ino == rootIno then Dirents.zero.enc() else []
+      requires fs.inode_types() == map ino: Ino {:trigger} :: if ino == rootIno then Inode.DirType else Inode.FileType
+      requires fs.fs.inode_owner() == map ino: Ino {:trigger} :: if ino == rootIno then Fs.Some(()) else Fs.None
       ensures Valid()
+      ensures data == map[rootIno := DirFile(map[])]
     {
-      fs := new ByteFilesys.Init(d);
-      dirents := map[];
-      data := map[];
+      this.fs := fs;
+      this.rootIno := rootIno;
+      var dirents0 : map<Ino, Dirents> := map[rootIno := Dirents.zero];
+      this.dirents := dirents0;
+      this.data := map[rootIno := DirFile(map[])];
+      new;
+      Dirents.zero_dir();
+      assert ValidData() by {
+        reveal ValidFiles();
+        reveal ValidDirs();
+      }
+    }
+
+    static method allocEmptyDir(fs: ByteFilesys<()>, txn: Txn) returns (ok: bool, ino: Ino)
+      modifies fs.Repr
+      requires fs.Valid() ensures ok ==> fs.Valid()
+      requires fs.fs.has_jrnl(txn)
+      requires forall ino:Ino :: fs.data()[ino] == []
+      ensures ok ==>
+      && fs.data() == old(fs.data()[ino := Dirents.zero.enc()])
+      && old(fs.fs.inode_owner()[ino].None?)
+      && fs.fs.inode_owner() == old(fs.fs.inode_owner()[ino := Some(())])
+      && fs.inode_types() == old(fs.inode_types()[ino := Inode.DirType])
+    {
+      ok, ino := fs.allocInode(txn, ());
+      var ino0 := ino;
+      if !ok {
+        return;
+      }
+
+      assert fs.Valid();
+
+      var i := fs.startInode(txn, ino);
+      i := fs.setType(ino, i, Inode.DirType);
+
+      var emptyDir := Dirents.zero.encode();
+      Dirents.zero.enc_len();
+      ok, i := fs.appendIno(txn, ino, i, emptyDir);
+      if !ok {
+        return;
+      }
+      assert fs.data()[ino] == Dirents.zero.enc();
+      fs.finishInode(txn, ino, i);
+      assert fs.Valid();
+    }
+
+    static method New(d: Disk) returns (fs: Option<DirFilesys>)
+      ensures fs.Some? ==> fresh(fs.x) && fs.x.Valid()
+      ensures fs.Some? ==> fs.x.data == map[fs.x.rootIno := DirFile(map[])]
+    {
+      var fs_ := new ByteFilesys.Init(d);
+
+      var txn := fs_.jrnl.Begin();
+      var ok, rootIno_ := allocEmptyDir(fs_, txn);
+      if !ok {
+        return None;
+      }
+      ok := txn.Commit();
+      if !ok {
+        return None;
+      }
+      assert fs_.Valid();
+
+      var dir_fs := new DirFilesys.Init(fs_, rootIno_);
+      return Some(dir_fs);
     }
   }
 }
