src/Dafny/examples/fs/block_fs.dfy
@@ -47,6 +47,7 @@ module BlockFs
   // public
   method New<InodeAllocState(!new)>(d: Disk) returns (fs: IndFilesys<InodeAllocState>)
     ensures fs.ValidQ()
+    ensures fresh(fs.Repr)
     ensures block_data(fs.data) == map ino: Ino {:trigger} :: InodeData.zero
     ensures fs.metadata == map ino: Ino {:trigger} :: Inode.Meta(0, Inode.FileType)
     ensures fs.inode_owner() == map ino: Ino {:trigger} :: Fs.None
